\documentclass{article}
\usepackage{epsfig}
\usepackage{amsmath}
\pagestyle{empty}
\begin{document}
$G(z) = \frac{Y(z)}{U(z)} = a_0 + a_1\,z^{-1} + a_2\,z^{-2} + \ldots + a_n\,z^{-n} $
\pagebreak

$a_i$
\pagebreak

$x(k+1) = A\,x(k) + B\,u(k)$
\pagebreak

$ y(k) = C\,x(k) + D\,u(k) $
\pagebreak

$A = \begin{pmatrix} 0 & 1 & 0 & \ldots & 0 \\ & & \ddots & & \\ & & & 0 & 1 \\ 0 & & \ldots & & 0 \end{pmatrix} $
\pagebreak

$B = \begin{pmatrix} 0 \\ \vdots \\ 0 \\ 1 \end{pmatrix} $
\pagebreak

$C = \begin{pmatrix} a_n & \ldots & a_2 & a_1 \end{pmatrix} $
\pagebreak

$D = \begin{pmatrix} a_0 \end{pmatrix} $
\pagebreak

$A$
\pagebreak

$B$
\pagebreak

$a_0,\,a_1,\,\ldots,\,a_n$
\pagebreak

$n$
\pagebreak

$n+1$
\pagebreak

\end{document}
